new base

src/NewBaseSystem.v
@@ -1,266 +1,194 @@
-Require Import Crypto.Util.Tactics.
-Require Import Crypto.Tactics.VerdiTactics.
-Require Import Crypto.Util.Decidable.
-Require Import Psatz.
-Require Import Coq.omega.Omega.
+Require Import Crypto.Util.Tactics Crypto.Util.Decidable.
 
+Require Import ZArith Nsatz Psatz Coq.omega.Omega.
 Require Import Coq.ZArith.BinIntDef. Local Open Scope Z_scope.
-Require Import Crypto.Algebra. Import Algebra.Ring.
 
 Require Coq.Lists.List. Local Notation list := List.list.
 Require Crypto.Util.Tuple. Local Notation tuple := Tuple.tuple.
-
-Import ZArith. (* for ring *)
 
     (* TODO: move *)
     Lemma fst_pair {A B} (a:A) (b:B) : fst (a,b) = a. reflexivity. Qed.
     Lemma snd_pair {A B} (a:A) (b:B) : snd (a,b) = b. reflexivity. Qed.
 
-    Program Definition add_to_nth {n} i x : tuple Z n -> tuple Z n :=
-      Tuple.on_tuple (ListUtil.update_nth i (Z.add x)) _.
-    Next Obligation. apply ListUtil.length_update_nth. Defined.
-
-    Lemma combine_update_nth_r {A B} (ls:list A) (rs:list B) i f :
-      List.combine ls (ListUtil.update_nth i f rs) =
-      ListUtil.update_nth i (fun p => (fst p, f (snd p))) (List.combine ls rs).
-    Admitted.
+    (* TODO: move to ListUtil *)
     Lemma update_nth_id {T} i (xs:list T) : ListUtil.update_nth i id xs = xs.
-    Admitted.
+    Proof.
+      revert xs; induction i; destruct xs; simpl; solve [ trivial | congruence ].
+    Qed.
+
     Lemma map_fst_combine {A B} (xs:list A) (ys:list B) : List.map fst (List.combine xs ys) = List.firstn (length ys) xs.
-    Admitted.
+    Proof.
+      revert xs; induction ys; destruct xs; simpl; solve [ trivial | congruence ].
+    Qed.
+
+    Lemma map_snd_combine {A B} (xs:list A) (ys:list B) : List.map snd (List.combine xs ys) = List.firstn (length xs) ys.
+    Proof.
+      revert xs; induction ys; destruct xs; simpl; solve [ trivial | congruence ].
+    Qed.
+
     Lemma nth_default_seq_inbouns d s n i (H:(i < n)%nat) :
       List.nth_default d (List.seq s n) i = (s+i)%nat.
     Proof.
       progress cbv [List.nth_default].
       rewrite ListUtil.nth_error_seq.
-      VerdiTactics.break_if; solve [ trivial | omega ].
+      break_match; solve [ trivial | omega ].
     Qed.
+
+Delimit Scope runtime_scope with RT.
+Definition runtime_mul := Z.mul. Global Infix "*" := runtime_mul : runtime_scope.
+Definition runtime_add := Z.add. Global Infix "+" := runtime_add : runtime_scope. 
 
 Module B.
-  Section NewBaseSystem.
-    Let limb := (Z*Z)%type. (* position coefficient and run-time value *)
-    Definition eval (p:list limb) : Z :=
-      List.fold_right Z.add 0%Z (List.map (fun t => fst t * snd t) p).
-    
-    Lemma eval_nil : eval nil = 0. Proof. reflexivity. Qed.
-    Lemma eval_cons p q : eval (p::q) = (fst p) * (snd p) + eval q. Proof. reflexivity. Qed.
-    Lemma eval_app p q: eval (p++q) = eval p + eval q.
-    Proof. induction p; simpl eval; rewrite ?eval_nil, ?eval_cons; nsatz. Qed.
+  Let limb := (Z*Z)%type. (* position coefficient and run-time value *)
+  Definition eval (p:list limb) : Z :=
+    List.fold_right Z.add 0%Z (List.map (fun t => fst t * snd t) p).
+  
+  Lemma eval_nil : eval nil = 0. Proof. reflexivity. Qed.
+  Lemma eval_cons p q : eval (p::q) = (fst p) * (snd p) + eval q. Proof. reflexivity. Qed.
+  Lemma eval_app p q: eval (p++q) = eval p + eval q.
+  Proof. induction p; simpl eval; rewrite ?eval_nil, ?eval_cons; nsatz. Qed.
 
-    Definition mul (p q:list limb) : list limb :=
-      List.flat_map (fun t => List.map (fun t' => (fst t * fst t', snd t * snd t')) q) p.
-    Lemma eval_map_mul a x q : eval (List.map (fun t => (a * fst t, x * snd t)) q) = a * x * eval q.
-    Proof. induction q; simpl List.map;
-             rewrite ?eval_nil, ?eval_cons, ?fst_pair, ?snd_pair; nsatz. Qed.
-    Lemma mul_correct p q : eval (mul p q) = eval p * eval q.
-    Proof. induction p; simpl mul;
-             rewrite ?eval_nil, ?eval_cons, ?eval_app, ?eval_map_mul; nsatz. Qed.
+  Definition mul (p q:list limb) : list limb :=
+    List.flat_map (fun t => List.map (fun t' => (fst t * fst t', (snd t * snd t')%RT)) q) p.
+  Lemma eval_map_mul a x q : eval (List.map (fun t => (a * fst t, x * snd t)) q) = a * x * eval q.
+  Proof. induction q; simpl List.map;
+           rewrite ?eval_nil, ?eval_cons, ?fst_pair, ?snd_pair; nsatz. Qed.
+  Lemma eval_mul p q : eval (mul p q) = eval p * eval q.
+  Proof. induction p; simpl mul;
+           rewrite ?eval_nil, ?eval_cons, ?eval_app, ?eval_map_mul; nsatz. Qed.
 
-    Section Positional.
-      Context (weight : nat -> Z) (* [weight i] is the weight of position [i] *)
-              (weight_0 : weight 0%nat = 1%Z)
-              (weight_nonzero : forall i, weight i <> 0).
+  Section GeneralizedMersenneReduction.
+    Fixpoint split (s:Z) (xs:list limb) : list limb * list limb :=
+      match xs with
+      | nil => (nil, nil)
+      | cons x xs' =>
+        let sxs' := split s xs' in
+        if dec (fst x mod s = 0)
+        then (fst sxs',          cons (fst x / s, snd x) (snd sxs'))
+        else (cons x (fst sxs'), snd sxs')
+      end.
 
-      Definition eval_positional {n:nat} (xs:tuple Z n) : Z :=
-        eval (List.combine (List.map weight (List.seq 0 n)) (Tuple.to_list n xs)).
+    Lemma eval_split s p (s_nonzero:s<>0) :
+      eval (fst (split s p)) + s * eval (snd (split s p)) = eval p.
+    Proof. induction p;
+             repeat match goal with
+                    | H:_ |- _ => unique pose proof (Z_div_exact_full_2 _ _ s_nonzero H)
+                    | _ => progress rewrite ?split_cons, ?eval_cons, ?fst_pair, ?snd_pair
+                    | _ => progress simpl split
+                    | _ => progress break_match
+                    | _ => nsatz
+                    end. Qed.
 
-      Lemma eval_positional_add_to_nth {n} (i:nat) (H:(i<n)%nat) (x:Z) (xs:tuple Z n) :
-        eval_positional (add_to_nth i x xs) = weight i * x + eval_positional xs.
-      Proof.
-        cbv [eval_positional add_to_nth Tuple.on_tuple]; rewrite !Tuple.to_list_from_list.
-        rewrite combine_update_nth_r at 1.
-        rewrite <-(update_nth_id i (List.combine _ _)) at 2.
-        rewrite <-!(ListUtil.splice_nth_equiv_update_nth_update _ _ (weight 0, 0)) by (autorewrite with distr_length; lia); progress cbv [ListUtil.splice_nth id].
-        repeat match goal with
-        | |- context[?w] => progress (replace w with (weight i); [ring|])
-        | _ => progress rewrite ?eval_app, ?eval_cons, ?fst_pair, ?snd_pair, <-?ListUtil.map_nth_default_always, ?map_fst_combine, ?List.firstn_all2, ?ListUtil.map_nth_default_always, ?nth_default_seq_inbouns by (autorewrite with distr_length; lia)
-        | _ => reflexivity
-        end.
-      Qed.
+    Definition reduce (s:Z) (c:list limb) (p:list limb) : list limb :=
+      let ab := split s p in fst ab ++ mul c (snd ab).
 
-      Fixpoint place (t:limb) (i:nat) : nat * Z :=
-        if dec (fst t mod weight i = 0)
-        then (i, fst t / weight i * snd t)
-        else match i with S i' => place t i' | O => (O, fst t * snd t) end.
+    Lemma reduction_rule a b s c (modulus_nonzero:s-c<>0) :
+      (a + s * b) mod (s - c) = (a + c * b) mod (s - c).
+    Proof. replace (a + s * b) with ((a + c*b) + b*(s-c)) by nsatz.
+           rewrite Z.add_mod, Z_mod_mult, Z.add_0_r, Z.mod_mod; trivial. Qed.
 
-      Lemma place_in_range (t:limb) (n:nat) : (fst (place t n) < S n)%nat.
-      Proof. induction n; simpl; VerdiTactics.break_match; simpl; omega. Qed.
+    Lemma eval_reduce s c p (s_nonzero:s<>0) (modulus_nonzero:s-eval c<>0) :
+      eval (reduce s c p) mod (s - eval c) = eval p mod (s - eval c).
+    Proof. cbv [reduce].
+           rewrite eval_app, eval_mul, <-reduction_rule, eval_split; trivial. Qed.
+  End GeneralizedMersenneReduction.
 
-      Lemma eval_place t i :
-        weight (fst (place t i)) * snd (place t i) = fst t * snd t.
-      Proof. induction i; simpl place; VerdiTactics.break_match;
-               try match goal with H:_ |- _ => pose proof (Z_div_exact_full_2 _ _ (weight_nonzero _) H) end;
-               rewrite ?weight_0, ?Z.div_1_r, ?fst_pair, ?snd_pair; nsatz. Qed.
+  Section Positional.
+    Context (weight : nat -> Z) (* [weight i] is the weight of position [i] *)
+            (weight_0 : weight 0%nat = 1%Z)
+            (weight_nonzero : forall i, weight i <> 0).
 
-      Definition place_all {n} (init:tuple Z n) (p:list limb) :=
-        List.fold_right (fun t => let p := place t (pred n) in add_to_nth (fst p) (snd p)) init p.
-      Lemma eval_positional_place_all {n} p (init:tuple Z n) (n_nonzero:n<>O) :
-        eval_positional (place_all init p) = eval p + eval_positional init.
-      Proof. induction p; simpl; try pose proof place_in_range a (pred n);
-               rewrite ?eval_positional_add_to_nth by omega;
-               rewrite ?eval_cons, ?eval_place; try nsatz. Qed.
+    Definition from_positional {n:nat} (xs:tuple Z n) : list limb :=
+      List.combine (List.map weight (List.seq 0 n)) (Tuple.to_list n xs).
 
-    Definition carry (from next : Z) (p : rep) : rep :=
-      let cap := (next / from)%Z in
-      flat_map (fun cx => let '(c,x) := cx in
-                          if dec (Logic.eq c from)
-                          then ((c, x mod cap) :: (next, x / cap) :: nil)%Z
-                          else ((c,x) :: nil)) p.
+    Program Definition add_to_nth {n} i x : tuple Z n -> tuple Z n :=
+      Tuple.on_tuple (ListUtil.update_nth i (runtime_add x)) _.
+    Next Obligation. apply ListUtil.length_update_nth. Defined.
 
-    Definition gather_or_leave b cx gso : rep * Z :=
-      if dec (Logic.eq ((fst cx) mod b) 0)%Z
-      then (fst gso, Z.add (((fst cx) / b) * (snd cx)) (snd gso)) (* TODO: use a compile-time scaling operation that compile-time checks whether the coefficient is 1 and skips multiplication if so. Maybe use notation scopes for compiletime and runtime. *)
-      else (cx :: fst gso, snd gso).
-
-    Definition gather_single (b : Z) (p : rep) : rep * Z :=
-      fold_right (gather_or_leave b) (nil,0) p.
-
-    Definition gather' (base:list Z) (p:rep) : (rep * list Z) :=
-      fold_right (fun b state =>
-                    let gso := gather_single b (fst state) in
-                    (fst gso, snd gso::snd state)) (p, nil) base.
-    Definition gather b p := snd (gather' b p).
-
-  (*
-    Let base := (1::10::100::1000::10000::100000::1000000::10000000::nil)%Z.
-    Axiom f0 f1 f2 f3 : R.
-    Axiom g0 g1 g2 g3 : R.
-    Let f_ := f0::f1::f2::f3::nil.
-    Let g_ := g0::g1::g2::g3::nil.
-
-    Let f := Eval compute in (combine base f_).
-    Let g := Eval compute in (combine base g_).
-
-    Local Infix "*" := ZRmul.
-    Compute gather base (mul f g).
-  *)
-    
-
-    Section Proofs.
-
-    Lemma add_correct p q : eval (add p q) = eval p + eval q. Proof. apply eval_app. Qed.
-
-    Lemma opp_correct p : eval (opp p) = - (eval p).
+    Lemma eval_positional_add_to_nth {n} (i:nat) (H:(i<n)%nat) (x:Z) (xs:tuple Z n) :
+      eval (from_positional (add_to_nth i x xs)) = weight i * x + eval (from_positional xs).
     Proof.
-      induction p; simpl opp;
-        rewrite ?eval_nil, ?eval_cons, ?fst_pair, ?snd_pair, ?IHp; ring.
+      cbv [from_positional add_to_nth Tuple.on_tuple]; rewrite !Tuple.to_list_from_list.
+      rewrite ListUtil.combine_update_nth_r at 1.
+      rewrite <-(update_nth_id i (List.combine _ _)) at 2.
+      rewrite <-!(ListUtil.splice_nth_equiv_update_nth_update _ _ (weight 0, 0)) by (autorewrite with distr_length; lia); progress cbv [ListUtil.splice_nth id].
+      repeat match goal with
+             | |- context[?w] => progress (replace w with (weight i); [ring|])
+             | _ => progress rewrite ?eval_app, ?eval_cons, ?fst_pair, ?snd_pair, <-?ListUtil.map_nth_default_always, ?map_fst_combine, ?List.firstn_all2, ?ListUtil.map_nth_default_always, ?nth_default_seq_inbouns, ?(eq_refl:runtime_add=Z.add) by (autorewrite with distr_length; lia)
+             | _ => reflexivity
+             end.
     Qed.
 
-    Lemma carry_correct from next: from <> 0 ->
-                                   next mod from = 0 ->
-                                   next / from <> 0 ->
-                                   forall p,
-                                      eval (carry from next p) = eval p.
-    Proof.
-      induction p; [reflexivity|]; intros; simpl carry; destruct_head prod.
-      break_match; subst; rewrite !eval_app, ?eval_cons, ?eval_nil;
-        rewrite IHp; [|ring].
-      simpl fst; simpl snd; ring_simplify.
-      match goal with |- ?a + ?b + ?x = ?c + ?x =>
-                      replace (a + b) with c; [ring|] end.
-      match goal with |- _ * ?x = _ * (?x mod ?y) + _ * (?x / ?y) =>
-                      rewrite (Z.div_mod x y) at 1 by auto end.
-      rewrite Z.mul_add_distr_l, !Z.mul_assoc.
-      rewrite <-Z_div_exact_full_2 by assumption. ring.
-    Qed.
+    Fixpoint place (t:limb) (i:nat) : nat * Z :=
+      if dec (fst t mod weight i = 0)
+      then (i, let c := fst t / weight i in (c * snd t)%RT)
+      else match i with S i' => place t i' | O => (O, fst t * snd t)%RT end.
 
-    Lemma gather_single_all p : Logic.eq (fst (gather_single 1%Z p)) nil.
-    Proof.
-      induction p; [solve [trivial]|]; simpl gather_single.
-      unfold gather_or_leave; rewrite Z.mod_1_r, IHp.
-      break_match; [reflexivity|congruence].
-    Qed.
+    Lemma place_in_range (t:limb) (n:nat) : (fst (place t n) < S n)%nat.
+    Proof. induction n; simpl; break_match; simpl; omega. Qed.
 
-    Lemma gather_all base' p : Logic.eq (fst (gather' (1%Z::base') p)) nil.
-    Proof. unfold gather'; simpl fst; setoid_rewrite gather_single_all; reflexivity. Qed.
+    Lemma eval_place t i :
+      weight (fst (place t i)) * snd (place t i) = fst t * snd t.
+    Proof. induction i; simpl place; break_match;
+             try match goal with H:_ |- _ => pose proof (Z_div_exact_full_2 _ _ (weight_nonzero _) H) end;
+             rewrite ?weight_0, ?Z.div_1_r, ?fst_pair, ?snd_pair; nsatz. Qed.
 
-    Lemma gather_single_correct b (b_nonzero : b <> 0%Z) p :
-      eval (fst (gather_single b p)) + (b * snd (gather_single b p)) = eval p.
-    Proof.
-      induction p; simpl; [rewrite ?eval_nil; ring|].
-      cbv [gather_or_leave]; destruct_head' prod; break_match; try congruence; simpl;
-        rewrite !eval_cons; simpl; rewrite <-IHp; simpl fst in *; [|ring].
-      rewrite Z.mul_add_distr_l, !Z.mul_assoc, <-Zdiv.Z_div_exact_full_2;
-        auto; ring.
-    Qed.
-
-    Lemma gather'_correct base : forall p, (forall b, In b base -> b <> 0%Z) ->
-      eval (fst (gather' base p)) + eval (combine base (snd (gather' base p))) = eval p.
-    Proof.
-      induction base; intros; simpl; [rewrite eval_nil; auto using right_identity|].
-      setoid_rewrite eval_cons. rewrite associative, gather_single_correct; auto using in_cons, in_eq.
-    Qed.
-
-    Lemma gather_correct base p : (forall b, In b base -> b <> 0%Z) ->
-      eval (combine (1%Z::base) (gather (1%Z::base) p)) = eval p.
-    Proof.
-      intros. etransitivity; [|eapply gather'_correct; eassumption].
-      simpl; setoid_rewrite eval_cons.
-      rewrite <-gather_single_correct with (p := fst (gather' base p)) (b := 1%Z) by congruence.
-      rewrite gather_single_all, eval_nil. simpl fst; simpl snd. ring.
-    Qed.
-
-    End Proofs.
-
-    Section Ring.
-
-    Definition eq (p q : rep) : Prop := eval p = eval q.
-
-    Definition zero : rep := nil.
-
-    Definition one : rep := ((1,1) :: nil).
-
-    Definition sub (p q : rep) : rep := add p (opp q).
-
-    Lemma sub_correct p q : eval (sub p q) = eval p - eval q.
-    Proof. cbv [sub]. rewrite add_correct, opp_correct. ring. Qed.
-
-    Lemma is_ring : @Algebra.ring rep eq zero one opp add sub mul.
-    Proof.
-      cbv [eq]; eapply (isomorphism_to_subring_ring (ringR := ring_Z) (phi := eval)).
-      Grab Existential Variables.
-      + reflexivity.
-      + reflexivity.
-      + apply mul_correct.
-      + apply sub_correct.
-      + apply add_correct.
-      + apply opp_correct.
-      + tauto.
-      + repeat intro. rewrite !mul_correct. congruence.
-      + repeat intro. rewrite !sub_correct. congruence.
-      + repeat intro. rewrite !add_correct. congruence.
-      + repeat intro. rewrite !opp_correct. congruence.
-      + intros; apply Z.eq_dec.
-      + econstructor; repeat intro; congruence.
-    Qed.
-    End Ring.
-
-    Section Split.
-      
-    Definition split coef p : rep * rep :=
-      fold_right (fun cx state =>
-                    if dec (fst cx < coef)
-                    then (cx :: fst state, snd state)
-                    else (fst state, (fst cx / coef, snd cx) :: snd state))
-                 (nil, nil) p.
-
-    Lemma split_correct coef p : coef <> 0 ->
-      (forall cx, In cx p -> fst cx < coef \/ (fst cx) mod coef = 0) ->
-      eval (fst (split coef p)) + coef * eval (snd (split coef p)) = eval p.
-    Proof.
-      induction p; intros; simpl; rewrite ?eval_nil, ?eval_cons; [ring|].
-      break_match; repeat (simpl fst; simpl snd; rewrite ?eval_cons);
-        rewrite <-IHp; auto using associative, in_cons.
-      ring_simplify.
-      rewrite <-Z_div_exact_full_2 by (auto;
-        match goal with H : forall cx, _ -> _ \/ _ |- _ =>
-                      destruct (H a); auto using in_eq; congruence
-        end).
-      destruct (split coef p); destruct a; simpl fst; simpl snd.
-      ring.
-    Qed.
-
-    End Split.
-
-  End NewBaseSystem.
+    Definition to_positional {n} (init:tuple Z n) (p:list limb) :=
+      List.fold_right (fun t => let p := place t (pred n) in add_to_nth (fst p) (snd p)) init p.
+    Lemma eval_from_positional_to_positional {n} p (init:tuple Z n) (n_nonzero:n<>O) :
+      eval (from_positional (to_positional init p)) = eval p + eval (from_positional init).
+    Proof. induction p; simpl; try pose proof place_in_range a (pred n);
+             rewrite ?eval_positional_add_to_nth by omega;
+             rewrite ?eval_cons, ?eval_place; try nsatz. Qed.
+  End Positional.
 End B.
+
+Local Coercion Z.of_nat : nat >-> Z.
+Import Coq.Lists.List.ListNotations. Local Open Scope list_scope.
+Program Definition zeros n : tuple Z n := Tuple.from_list n (List.map (fun _ => 0) (List.seq 0 n)) _.
+Next Obligation. rewrite List.map_length, List.seq_length; reflexivity. Qed.
+
+Goal let base10 i := 10^i in forall f0 f1 f2 f3 g0 g1 g2 g3 : Z, False. intros.
+  let t := constr:(B.to_positional base10 (zeros 7)
+                                   (B.mul
+                                      (B.from_positional base10 (Tuple.from_list _ [f0;f1;f2;f3] eq_refl))
+                                      (B.from_positional base10 (Tuple.from_list _ [g0;g1;g2;g3] eq_refl)))) in
+  let t := (eval cbv -[runtime_mul runtime_add] in t) in
+  let t := (eval cbv [runtime_mul runtime_add] in t) in
+  remember t eqn:Heqt; rewrite !Z.mul_1_l, !Z.add_0_r, !Z.add_assoc in Heqt.
+Abort.
+
+Goal let base2_51 i := 2 ^ (51 * i) in forall f0 f1 f2 f3 f4 g0 g1 g2 g3 g4 : Z, False. intros.
+  let t := constr:(B.to_positional base2_51 (zeros 5)
+                                   (B.reduce (2^255) [(1,19)] 
+                                   (B.mul
+                                      (B.from_positional base2_51 (Tuple.from_list _ [f0;f1;f2;f3;f4] eq_refl))
+                                      (B.from_positional base2_51 (Tuple.from_list _ [g0;g1;g2;g3;g4] eq_refl))))) in
+  let t := (eval cbv -[runtime_mul runtime_add] in t) in
+  let t := (eval cbv [runtime_mul runtime_add] in t) in
+  remember t eqn:Heqt; rewrite !Z.mul_1_l, !Z.add_0_r, !Z.add_assoc, !Z.mul_assoc in Heqt.
+Abort.
+
+
+Goal let base2_25_5 i := 2 ^ (25 * (i / 2) + 26 * (i - i / 2)) in forall f0 f1 f2 f3 f4 f5 f6 f7 f8 f9 g0 g1 g2 g3 g4 g5 g6 g7 g8 g9: Z, False. intros.
+  let t := constr:(B.to_positional base2_25_5 (zeros 10)
+                                   (B.reduce (2^255) [(1,19)] 
+                                   (B.mul
+                                      (B.from_positional base2_25_5 (Tuple.from_list _ [f0;f1;f2;f3;f4;f5;f6;f7;f8;f9] eq_refl))
+                                      (B.from_positional base2_25_5 (Tuple.from_list _ [g0;g1;g2;g3;g4;g5;g6;g7;g8;g9] eq_refl))))) in
+  let t := (eval cbv -[runtime_mul runtime_add] in t) in
+  let t := (eval cbv [runtime_mul runtime_add] in t) in
+  remember t eqn:Heqt; rewrite !Z.mul_1_l, !Z.add_0_r, !Z.add_assoc, !Z.mul_assoc in Heqt.
+Abort.
+
+Goal let base2_56 i := 2 ^ (56 * i) in forall f0 f1 f2 f3 f4 f5 f6 f7 g0 g1 g2 g3 g4 g5 g6 g7: Z, False. intros.
+  let t := constr:(B.to_positional base2_56 (zeros 8)
+                                   (B.reduce (2^448) [(2^224,1);(1,-1)] 
+                                   (B.reduce (2^448) [(2^224,1);(1,-1)] 
+                                   (B.mul
+                                      (B.from_positional base2_56 (Tuple.from_list _ [f0;f1;f2;f3;f4;f5;f6;f7] eq_refl))
+                                      (B.from_positional base2_56 (Tuple.from_list _ [g0;g1;g2;g3;g4;g5;g6;g7] eq_refl)))))) in
+  let t := (eval cbv -[runtime_mul runtime_add] in t) in
+  let t := (eval cbv [runtime_mul runtime_add] in t) in
+  remember t eqn:Heqt; rewrite !Z.mul_1_l, !Z.add_0_r, !Z.add_assoc, !Z.mul_assoc, !Z.mul_opp_l, !Z.add_opp_r in Heqt.
+Abort.
